 \documentclass[onecolumn]{aastex63}
\usepackage{amsmath}
\usepackage{listings}
\usepackage{tensor}

\lstset{frame=tb,
  language=Python,
  showstringspaces=false,
  columns=flexible,
  basicstyle={\small\ttfamily},
  commentstyle={\small\ttfamily},
  breaklines=true,
  breakatwhitespace=true,
  tabsize=4
}

\usepackage[T1]{fontenc}
\newcommand{\vdag}{(v)^\dagger}
\newcommand\aastex{AAS\TeX}
\newcommand\latex{La\TeX}
\shortauthors{McClellan}
\graphicspath{{./}{figures/}}


\begin{document}

\title{Scratch Work}
\author{B. Connor McClellan}
\affiliation{University of Virginia}
\keywords{}

\setlength\parindent{0pt}

\section{Closed-Form Solutions for Ly$\alpha$ Resonant Scattering}

$x$ is related to the frequency variable $\sigma$ by 

\begin{equation} \label{sigma}
    \sigma = \frac{\sqrt{2\pi^2/27}}{a} x^3
\end{equation}

The Voigt function line profile is defined as 

\begin{equation} \label{lineprofile}
    \phi = \frac{a}{\sqrt{\pi} x^2}
\end{equation}

and

\begin{equation}
    R\kappa_0 = \tau_0
\end{equation}

Equation C17 in \citet{2006ApJ...649...14D} reads

\begin{equation} \label{dijkstra}
    J(x) = \frac{\sqrt{\pi}}{\sqrt{24}a\tau_0}\left(\frac{x^2}{1 + \cosh{\sqrt{2\pi^3/27}(|x^3|/a\tau_0)}}\right)
\end{equation}

This will be checked against the boundary condition

\begin{equation}
    J = \sqrt{3} H
\end{equation}

by evaluating the surface flux derived from their Eq. C12. This equation reads 

\begin{equation} \label{c12}
    J(r, \sigma) = \frac{\sqrt{6}}{16 \pi^2 R} \frac{\kappa_0}{rr_s} \sum_{n=1}^{\infty}\sin(\lambda_n r) \sin(\lambda_n r_s) \frac{\exp{(-\lambda_n |\sigma|/\kappa_0)}}{\lambda_n}
\end{equation}

with

\begin{equation} \label{lambdan}
    \lambda_n = \frac{n\pi}{R}
\end{equation}

at lowest order. To find the flux, we calculate the following derivative.

\begin{equation}
    \begin{split}
    H(r, \sigma) &= \frac{1}{3\kappa_0 \phi}\frac{\partial J}{\partial r}\\
    &= \frac{1}{3\kappa_0 \phi}\frac{\partial}{\partial r}\left(\frac{\sqrt{6}}{16 \pi^2 R} \frac{\kappa_0}{rr_s} \sum_{n=1}^{\infty}\sin(\lambda_n r) \sin(\lambda_n r_s) \frac{\exp{(-\lambda_n |\sigma|/\kappa_0)}}{\lambda_n}\right)
    \end{split}
\end{equation}

Applying the product rule within the sum, we obtain

\begin{equation}
    H(r, \sigma) = \frac{1}{3 \phi} \frac{\sqrt{6}}{16 \pi^2 R} \frac{1}{r_s} \sum_{n=1}^{\infty} \sin(\lambda_n r_s) \frac{\exp{(-\lambda_n |\sigma|/\kappa_0)}}{\lambda_n} \left[ \frac{-\sin(\lambda_n r)}{r^2} + \frac{\lambda_n \cos(\lambda_n r)}{r}\right]
\end{equation}

At this point, the expression is evaluated at the surface, $r=R$. Eq. \ref{lambdan} is substituted in for $\lambda_n$.

\begin{equation}
    H(\sigma) = \frac{1}{3 \phi} \frac{\sqrt{6}}{16 \pi^2 R} \frac{1}{r_s} \sum_{n=1}^{\infty} \sin{\left(\frac{n\pi r_s}{R}\right)} \frac{\exp{(-n \pi |\sigma|/R\kappa_0)}}{\left(\frac{n\pi}{R}\right)} \left[ \frac{-\sin(n \pi)}{R^2} + \frac{n \pi \cos(n \pi)}{R^2}\right]
\end{equation}

The $\sin(n\pi)$ terms evaluate to zero, and the $\cos(n\pi)$ terms are equivalent to $(-1)^n$. We now have

\begin{equation}
    H(\sigma) = \frac{1}{3 \phi} \frac{\sqrt{6}}{16 \pi^2 R^2} \frac{1}{r_s} \sum_{n=1}^{\infty} (-1)^n \sin{\left(\frac{n\pi r_s}{R}\right)} \exp{(-n \pi |\sigma|/R\kappa_0)}
\end{equation}


\bibliography{bibliography}{}
\bibliographystyle{aasjournal}

\end{document}
